\documentclass{article}
\usepackage{amsmath}
\usepackage{amsfonts}
\usepackage{amssymb}
\begin{document}
\section*{Problem Set 3}

\subsection*{Problem 1}

\noindent
Given the Fibonacci number $F_n$ is its n-th term, prove
\begin{equation}
    F_n = \frac{p^n - q^n}{\sqrt{5}}
\end{equation}
where,
\begin{align}
    p &= \frac{1+\sqrt{5}}{2}\\
    q &= \frac{1-\sqrt{5}}{2}
\end{align}

\noindent
Proof by strong induction.\\
First, the base case $F_0$ and $F_1$ must be verified.
\begin{align*}
    F_0 &= \frac{p^0 - q^0}{\sqrt{5}}\\
        &= \frac{1 - 1}{\sqrt{5}}\\
        &= 0\\
        \\
    F_1 &= \frac{p^1 - q^1}{\sqrt{5}}\\
        &= \frac{ (\frac{1+\sqrt{5}}{2}) - (\frac{1-\sqrt{5} }{2})}{\sqrt{5}}\\
        &= \frac{\frac{2\sqrt{5}}{2}}{\sqrt{5}}\\
        &= 1\\
\end{align*}
Suppose $F_0,F_1,\ldots,F_n$ is true. Then $F_{n+1}$ must be true.
\begin{align*}
    F_{n+1} &= F_n + F_{n-1}\\
            &= \frac{p^n - q^n}{\sqrt{5}} + \frac{p^{n-1} - q^{n-1}}{\sqrt{5}}\\
            &= \frac{p^n(1+p^{-1}) - (q^n(1+q^{-1}))}{\sqrt{5}}\\
            &= \frac{p^n \cdot p - q^n \cdot q}{\sqrt{5}}\\
            &= \frac{p^{n+1} - q^{n+1}}{\sqrt{5}}\\
\end{align*}
So, (1) holds for all $n \in \mathbb{N}$. QED

\subsection*{Problem 2}

\subsection*{Problem 3}
\begin{align*}
    f &: A \rightarrow B\\
    g &: B \rightarrow C\\
    h &: A \rightarrow C\\
\end{align*}
($f$ and $g$ are both functions.)\\
\smallskip
(a) If h is surjective, then f must be surjective.\\
If h is surjective,
\begin{equation}
    (\#arrows\ of\ f) \ge |C|
\end{equation}
is true. Because f is function,
\begin{equation}
    |B| \ge (\#arrows\ of\ f)
\end{equation}
is also true. Then f must be surjective function. $\square$\\ 
(b) If h is surjective, then g must be surjective.\\
If g is injective function, still holds the lefthand side of the proposition. By the contradiction, it is false.\\
(c) If h is injective, then f must be injective.\\
If h is injective,\\
\begin{equation}
    (\#arrows\ of \ f) \le |C|
\end{equation}
iff f is injective. (c) is true.\\
(d) If h is injective and f is total, then g must be injective.\\


\end{document}